fairness/lawyer/examples/eo/eo_adequacy.v
@@ -1,0 +1,54 @@
+From iris.algebra Require Import auth gmap gset excl excl_auth.
+From iris.proofmode Require Import tactics.
+From trillium.fairness Require Import locales_helpers comp_utils trace_lookup fairness.
+From trillium.fairness.heap_lang Require Import simulation_adequacy notation.
+From trillium.fairness.lawyer Require Import counter_model sub_action_em.
+
+
+Definition eo_prog: val.
+Admitted. 
+
+Definition eo_ex_progress (l: loc) (extr : heap_lang_extrace) :=
+  ∀ (i: nat), ∃ n c, extr S!! n = Some c /\ heap (c.2) !! l = Some #i. 
+
+Definition eo_ex_mono (l: loc) (extr : heap_lang_extrace) :=
+  ∀ n, ∃ c c' oτ (i j: nat),
+    extr !! n = Some (c, Some (oτ, c')) /\
+    heap c.2 !! l = Some #i /\
+    heap c'.2 !! l = Some #j /\
+    i <= j
+.
+
+Section EOAdequacy.
+
+  Definition eoΣ: gFunctors.
+  Admitted. 
+
+  Theorem eo_progress
+    (l: loc)
+    (extr : heap_lang_extrace)
+    (Hexfirst : trfirst extr = ([eo_prog #0], {| heap := {[l:=#0]}; used_proph_id := ∅ |})):
+    (* (∀ tid, fair_ex tid extr) -> terminating_trace extr. *)
+    extrace_fairly_terminating extr. 
+  Proof using.
+    assert (heapGpreS eoΣ EM) as HPreG.
+    { apply _. }
+
+    destruct (trfirst extr) as [tp_ σ1] eqn:EX0. simpl in *. subst tp_.                
+    
+    set (s1 := init_om_state (EO_OP LIM) (trfirst extr)). 
+    
+    unshelve epose proof (simple_om_simulation_adequacy_terminate (EO_OP LIM) eofinΣ NotStuck
+                  _ _ _ _
+                  _ _ EX0) as FAIR_TERM; eauto.
+    { exact tt. }
+    { simpl. subst s1. rewrite EX0. apply init_om_state_init. }
+    
+    apply FAIR_TERM.
+    red. intros ?. iStartProof. iIntros "[HEAP INIT] !>".
+    iSplitL.
+    - admit.
+    - subst s1. rewrite EX0. iApply om_sim_RAH. 
+  Admitted. 
+
+End EOAdequacy.
